Improve Equiv.

theories/Equiv/Sim.v
@@ -4,7 +4,7 @@ Require Export paco3 SmallStepRelations StateType.
 Set Implicit Arguments.
 Unset Printing Records.
 
-(** * Simulation *)
+(** * Parametric Definition of Simulation and Bisimulation *)
 (** A characterization of simulation equivalence on states;
 works only for internally deterministic semantics *)
 
@@ -16,53 +16,14 @@ Definition isBisim t :=
   | Bisim => true
   end.
 
-CoInductive sim {S} `{StateType S} {S'} `{StateType S'}  : simtype -> S -> S' -> Prop :=
-  | simSilent t (σ1 σ1':S) (σ2 σ2':S') : (* result σ1 = result σ2 -> *)
-      plus2 step σ1 nil σ1'
-      -> plus2 step σ2 nil σ2'
-      -> sim t σ1' σ2'
-      -> sim t σ1 σ2
-  | simExtern t (pσ1 σ1:S) (pσ2 σ2:S') : (* result σ1 = result σ2 -> *)
-      star2 step pσ1 nil σ1
-      -> star2 step pσ2 nil σ2
-      -> activated σ1
-      -> activated σ2
-      -> (forall evt σ1', step σ1 evt σ1' -> exists σ2', step σ2 evt σ2' /\ sim t σ1' σ2')
-      -> (forall evt σ2', step σ2 evt σ2' -> exists σ1', step σ1 evt σ1' /\ sim t σ1' σ2')
-      -> sim t pσ1 pσ2
-  | simErr (σ1 σ1':S) (σ2:S')
-    : result σ1' = None
-      -> star2 step σ1 nil σ1'
-      -> normal2 step σ1'
-      -> sim Sim σ1 σ2
-  | simTerm t (σ1 σ1':S) (σ2 σ2':S')
-    : result σ1' = result σ2'
-      -> star2 step σ1 nil σ1'
-      -> star2 step σ2 nil σ2'
-      -> normal2 step σ1'
-      -> normal2 step σ2'
-      -> sim t σ1 σ2.
-
-Arguments sim [S] {H} [S'] {H0} _ _ _.
-
-Lemma sim_refl {S} `{StateType S} t (σ:S)
-      : sim t σ σ.
-Proof.
-  revert σ. cofix.
-  intros. destruct (step_dec σ) as [[[] []]|].
-  - eapply simExtern; intros; eauto using star2_refl; eexists; eauto.
-  - eapply simSilent; eauto using plus2O.
-  - eapply simTerm; eauto using star2_refl.
-Qed.
-
 Inductive sim_gen
           {S} `{StateType S} {S'} `{StateType S'} (r: simtype -> S -> S' -> Prop)  : simtype -> S -> S' -> Prop :=
-  | sim'Silent t (σ1 σ1':S) (σ2 σ2':S') : (* result σ1 = result σ2 -> *)
+  | SimSilent t (σ1 σ1':S) (σ2 σ2':S') : (* result σ1 = result σ2 -> *)
       plus2 step σ1 nil σ1'
       -> plus2 step σ2 nil σ2'
       -> r t σ1' σ2'
       -> sim_gen r t σ1 σ2
-  | sim'Extern t (pσ1 σ1:S) (pσ2 σ2:S') : (* result σ1 = result σ2 -> *)
+  | SimExtern t (pσ1 σ1:S) (pσ2 σ2:S') : (* result σ1 = result σ2 -> *)
       star2 step pσ1 nil σ1
       -> star2 step pσ2 nil σ2
       -> activated σ1
@@ -70,12 +31,12 @@ Inductive sim_gen
       -> (forall evt σ1', step σ1 evt σ1' -> exists σ2', step σ2 evt σ2' /\ r t σ1' σ2')
       -> (forall evt σ2', step σ2 evt σ2' -> exists σ1', step σ1 evt σ1' /\ r t σ1' σ2')
       -> sim_gen r t pσ1 pσ2
-  | sim'Err (σ1 σ1':S) (σ2:S')
+  | SimErr (σ1 σ1':S) (σ2:S')
     : result σ1' = None
       -> star2 step σ1 nil σ1'
       -> normal2 step σ1'
       -> sim_gen r Sim σ1 σ2
-  | sim'Term t (σ1 σ1':S) (σ2 σ2':S')
+  | SimTerm t (σ1 σ1':S) (σ2 σ2':S')
     : result σ1' = result σ2'
       -> star2 step σ1 nil σ1'
       -> star2 step σ2 nil σ2'
@@ -87,13 +48,13 @@ Arguments sim_gen [S] {H} [S'] {H0} r _ _ _.
 
 Hint Constructors sim_gen.
 
-Definition sim' {S} `{StateType S} {S'} `{StateType S'} t  (σ1:S) (σ2:S')
+Definition sim_bot {S} `{StateType S} {S'} `{StateType S'} t  (σ1:S) (σ2:S')
   := paco3 (@sim_gen S _ S' _) bot3 t σ1 σ2.
-Hint Unfold sim'.
+Hint Unfold sim_bot.
 
-Definition sim'r {S} `{StateType S} {S'} `{StateType S'} r t (σ1:S) (σ2:S')
+Definition sim {S} `{StateType S} {S'} `{StateType S'} r t (σ1:S) (σ2:S')
   := paco3 (@sim_gen S _ S' _) r t σ1 σ2.
-Hint Unfold sim'r.
+Hint Unfold sim.
 
 Lemma sim_gen_mon {S} `{StateType S} {S'} `{StateType S'}
 : monotone3 (@sim_gen S _ S' _).
@@ -108,46 +69,15 @@ Arguments sim_gen_mon [S] {H} [S'] {H0} [x0] [x1] [x2] r r' IN LE.
 
 Hint Resolve sim_gen_mon : paco.
 
-Lemma sim_sim' {S} `{StateType S} {S'} `{StateType S'} t (σ1:S) (σ2:S')
-: sim t σ1 σ2 -> sim' t σ1 σ2.
+Lemma sim_refl {S} `{StateType S} (σ:S) t r
+      : sim r t σ σ.
 Proof.
-  revert σ1 σ2. pcofix CIH.
-  intros. pfold.
-  inv H2; eauto using sim_gen.
-  - econstructor 2; eauto; intros.
-    + edestruct H6; eauto; dcr. eexists; eauto.
-    + edestruct H7; eauto; dcr. eexists; eauto.
-Qed.
-
-
-Lemma sim'_sim {S} `{StateType S} {S'} `{StateType S'} t (σ1:S) (σ2:S')
-: sim' t σ1 σ2 -> sim t σ1 σ2.
-Proof.
-  revert t σ1 σ2. cofix CIH.
-  intros.
-  assert (sim_gen (paco3 (@sim_gen S _ S' _) bot3 \3/ bot3) t σ1 σ2).
-  punfold H1.
-  destruct H2. destruct H4.
-  - econstructor; eauto.
-  - exfalso; intuition.
-  - econstructor 2; eauto; intros.
-    + edestruct H6; eauto; dcr. destruct H11. eexists; eauto. exfalso; intuition.
-    + edestruct H7; eauto; dcr. destruct H11. eexists; eauto. exfalso; intuition.
-  - econstructor 3; eauto.
-  - econstructor 4; eauto.
-Qed.
-
-Lemma sim'_refl {S} `{StateType S} (σ:S) t
-      : sim' t σ σ.
-Proof.
-  eapply sim_sim'. eapply sim_refl.
-Qed.
-
-Lemma sim'r_refl {S} `{StateType S} (σ:S) t r
-      : sim'r r t σ σ.
-Proof.
-  eapply paco3_mon. eapply sim'_refl.
-  isabsurd.
+  revert σ.
+  pcofix CIH.
+  intros. destruct (step_dec σ) as [[[] []]|].
+  - pfold. eapply SimExtern; intros; eauto using star2_refl; eexists; eauto.
+  - pfold. eapply SimSilent; eauto using plus2O.
+  - pfold. eapply SimTerm; eauto using star2_refl.
 Qed.
 
 Lemma sim_Y_left S `{StateType S} S' `{StateType S'} r t σA1 σB1 σ1' σ2
@@ -180,12 +110,12 @@ Ltac contr_trans :=
               rename H'' into H
           end).
 
-Lemma sim'_expansion_closed {S} `{StateType S}
+Lemma sim_expansion_closed {S} `{StateType S}
       (σ1 σ1':S) {S'} `{StateType S'} (σ2 σ2':S') r t
-  : sim'r r t σ1' σ2'
+  : sim r t σ1' σ2'
     -> star2 step σ1 nil σ1'
     -> star2 step σ2 nil σ2'
-    -> sim'r r t σ1 σ2.
+    -> sim r t σ1 σ2.
 Proof.
   intros SIM ? ?.
   pinversion SIM; subst; pfold;
@@ -195,11 +125,11 @@ Qed.
 Tactic Notation "size" "induction" hyp(n) :=
   pattern n; eapply size_induction with (f:=id); intros; unfold id in *.
 
-Lemma sim'_reduction_closed_1 t {S} `{StateType S}
+Lemma sim_reduction_closed_1 t {S} `{StateType S}
       (σ1 σ1':S) {S'} `{StateType S'} (σ2:S')
-  : sim' t σ1 σ2
+  : sim bot3 t σ1 σ2
     -> star2 step σ1 nil σ1'
-    -> sim' t σ1' σ2.
+    -> sim bot3 t σ1' σ2.
 Proof.
   intros Sim Star. eapply star2_star2n in Star. destruct Star as [n StarN].
   revert σ1 σ1' σ2 Sim StarN.
@@ -208,9 +138,9 @@ Proof.
   - invc StarN; eauto; relsimpl.
     eapply star2_star2n in H2. destruct H2 as [n' H2].
     edestruct (star2n_reach H9 H2); eauto. eapply H.
-    + eapply sim'_expansion_closed; eauto using star2n_star2, plus2_star2.
+    + eapply sim_expansion_closed; eauto using star2n_star2, plus2_star2.
     + eapply H1; try eapply H9. omega.
-      eapply sim'_expansion_closed;
+      eapply sim_expansion_closed;
       eauto using star2n_star2, plus2_star2.
   - eapply star2n_star2 in StarN; relsimpl; eauto.
   - pfold. eapply star2n_star2 in StarN; relsimpl; eauto.
@@ -218,11 +148,11 @@ Proof.
 Qed.
 
 
-Lemma sim'_reduction_closed_2 t {S} `{StateType S}
+Lemma sim_reduction_closed_2 t {S} `{StateType S}
       (σ1:S) {S'} `{StateType S'} (σ2 σ2':S')
-  : sim' t σ1 σ2
+  : sim bot3 t σ1 σ2
     -> star2 step σ2 nil σ2'
-    -> sim' t σ1 σ2'.
+    -> sim bot3 t σ1 σ2'.
 Proof.
   intros. eapply star2_star2n in H2. destruct H2 as [n ?].
   revert σ1 σ2' σ2 H1 H2.
@@ -232,10 +162,10 @@ Proof.
   - inv H3; eauto.
     eapply plus2_plus2n in H5. destruct H5. eapply plus2n_star2n in H5.
     edestruct (star2n_reach H3 H5); eauto. eapply H0.
-    + eapply sim'_expansion_closed. eapply H6.
+    + eapply sim_expansion_closed. eapply H6.
       eauto using plus2_star2. eauto using star2n_star2.
     + eapply H1; try eapply H9. omega.
-      eapply sim'_expansion_closed. eapply H6.
+      eapply sim_expansion_closed. eapply H6.
       eauto using plus2_star2. eapply star2_refl.
   - eapply star2n_star2 in H3. eapply activated_star_reach in H3; eauto.
   - pfold. eauto.
@@ -243,26 +173,26 @@ Proof.
     eapply star2_reach_normal in H3; eauto. eapply H0.
 Qed.
 
-Lemma sim'_reduction_closed t {S} `{StateType S}
+Lemma sim_reduction_closed t {S} `{StateType S}
       (σ1 σ1':S) {S'} `{StateType S'} (σ2 σ2':S')
-  : sim' t σ1 σ2
+  : sim bot3 t σ1 σ2
     -> star2 step σ1 nil σ1'
     -> star2 step σ2 nil σ2'
-    -> sim' t σ1' σ2'.
+    -> sim bot3 t σ1' σ2'.
 Proof.
   intros.
-  eapply sim'_reduction_closed_1; [| eauto].
-  eapply sim'_reduction_closed_2; eauto.
+  eapply sim_reduction_closed_1; [| eauto].
+  eapply sim_reduction_closed_2; eauto.
 Qed.
 
 
 
-Lemma sim'_terminate t {S1} `{StateType S1} (σ1 σ1':S1)
+Lemma sim_terminate t {S1} `{StateType S1} (σ1 σ1':S1)
       {S2} `{StateType S2} (σ2:S2)
 : star2 step σ1 nil σ1'
   -> normal2 step σ1'
   -> result σ1' <> None
-  -> sim' t σ1 σ2
+  -> sim bot3 t σ1 σ2
   -> exists σ2', star2 step σ2 nil σ2' /\ normal2 step σ2' /\ result σ1' = result σ2'.
 Proof.
   intros. general induction H1.
@@ -276,15 +206,15 @@ Proof.
       eexists; split; eauto.
   - relsimpl.
     eapply IHstar2; eauto.
-    eapply sim'_reduction_closed_1; eauto using star2, star2_silent.
+    eapply sim_reduction_closed_1; eauto using star2, star2_silent.
 Qed.
 
 
-Lemma sim'_terminate_2 t {S1} `{StateType S1} (σ2 σ2':S1)
+Lemma sim_terminate_2 t {S1} `{StateType S1} (σ2 σ2':S1)
       {S2} `{StateType S2} (σ1:S2)
 : star2 step σ2 nil σ2'
   -> normal2 step σ2'
-  -> sim' t σ1 σ2
+  -> sim bot3 t σ1 σ2
   -> exists σ1', star2 step σ1 nil σ1' /\ normal2 step σ1' /\
            (result σ1' = result σ2' \/ result σ1' = None).
 Proof.
@@ -299,23 +229,23 @@ Proof.
       * exfalso. eapply H2. eexists; eauto.
   - relsimpl.
     eapply IHstar2; eauto.
-    eapply sim'_reduction_closed_2; eauto using star2, star2_silent.
+    eapply sim_reduction_closed_2; eauto using star2, star2_silent.
 Qed.
 
-Lemma sim'_activated t {S1} `{StateType S1} (σ1:S1)
+Lemma sim_activated t {S1} `{StateType S1} (σ1:S1)
       {S2} `{StateType S2} (σ2:S2)
 : activated σ1
-  -> sim' t σ1 σ2
+  -> sim bot3 t σ1 σ2
   -> exists σ2', star2 step σ2 nil σ2' /\ activated σ2' /\
            ( forall (evt : event) (σ1'' : S1),
                step σ1 evt σ1'' ->
                exists σ2'' : S2,
-                 step σ2' evt σ2'' /\ sim' t σ1'' σ2'')
+                 step σ2' evt σ2'' /\ sim bot3 t σ1'' σ2'')
            /\
            ( forall (evt : event) (σ2'' : S2),
                step σ2' evt σ2'' ->
                exists σ1' : S1,
-                 step σ1 evt σ1' /\ sim' t σ1' σ2'').
+                 step σ1 evt σ1' /\ sim bot3 t σ1' σ2'').
 Proof.
   intros.
   pinversion H2; subst.
@@ -330,21 +260,21 @@ Proof.
   - exfalso. refine (activated_normal_star _ H1 _ _); eauto using star2.
 Qed.
 
-Lemma sim'_activated_2 t {S1} `{StateType S1} (σ1:S1)
+Lemma sim_activated_2 t {S1} `{StateType S1} (σ1:S1)
       {S2} `{StateType S2} (σ2:S2)
 : activated σ1
-  -> sim' t σ2 σ1
+  -> sim bot3 t σ2 σ1
   -> exists σ2', star2 step σ2 nil σ2' /\
            (activated σ2' /\
            ( forall (evt : event) (σ1'' : S1),
                step σ1 evt σ1'' ->
                exists σ2'' : S2,
-                 step σ2' evt σ2'' /\ (sim' t σ2'' σ1''))
+                 step σ2' evt σ2'' /\ (sim bot3 t σ2'' σ1''))
            /\
            ( forall (evt : event) (σ2'' : S2),
                step σ2' evt σ2'' ->
                exists σ1' : S1,
-                 step σ1 evt σ1' /\ (sim' t σ2'' σ1'))
+                 step σ1 evt σ1' /\ (sim bot3 t σ2'' σ1'))
            \/ (normal2 step σ2' /\ result σ2' = None)).
 Proof.
   intros.
@@ -380,13 +310,13 @@ Qed.
 
 Ltac zsimpl_step :=
   match goal with
-  | [ SIM : sim' ?t ?σ2 ?σ1, ACT : normal2 step ?σ2', STAR: star2 step ?σ2 nil ?σ2' |- _ ] =>
-    eapply sim'_reduction_closed_1 in SIM; [| eapply STAR]
+  | [ SIM : sim bot3 ?t ?σ2 ?σ1, ACT : normal2 step ?σ2', STAR: star2 step ?σ2 nil ?σ2' |- _ ] =>
+    eapply sim_reduction_closed_1 in SIM; [| eapply STAR]
   | [ SIM : paco3 (@sim_gen _ _ _ _) _ ?t ?σ2 ?σ1, ACT : normal2 step ?σ2', STAR: star2 step ?σ2 nil ?σ2' |- _ ] =>
-    eapply sim'_reduction_closed_1 in SIM; [| eapply STAR]
+    eapply sim_reduction_closed_1 in SIM; [| eapply STAR]
   | [ SIM : paco3 (@sim_gen _ _ _ _) _ ?t ?σ1 ?σ2,
             ACT : activated ?σ1', STAR: star2 step ?σ1 nil ?σ1' |- _ ] =>
-    eapply sim'_reduction_closed_1 in SIM; [| eapply STAR]
+    eapply sim_reduction_closed_1 in SIM; [| eapply STAR]
   | [ H : star2 ?R ?σ1 nil ?σ2, H':plus2 ?R ?σ2 nil ?σ3 |- _ ] =>
     eapply (star2_plus2_plus2 H) in H'; clear H; simpl in H'
   | [ H : plus2 ?R ?σ1 nil ?σ2, H':star2 ?R ?σ2 nil ?σ3 |- _ ] =>
@@ -407,7 +337,7 @@ Ltac zsimpl_step :=
           step ?σ1 evt σ2'' -> _ |- _ ] => specialize (A _ _ H); dcr
   | [ H : _ \/ bot3 _ _ _ |- _ ] => destruct H;[ | isabsurd]
   | [ SIM : paco3 (@sim_gen _ _ _ _) _ ?t ?σ1 ?σ2, ACT : activated ?σ2', STAR: star2 step ?σ2 nil ?σ2' |- _ ] =>
-    eapply sim'_reduction_closed_2 in SIM; [| eapply STAR]
+    eapply sim_reduction_closed_2 in SIM; [| eapply STAR]
   | [ H : plus2 step ?σ nil _, H' : star2 (@step ?S ?ST) ?σ _ ?σ',
                                     H'' : normal2 _ ?σ' |- _ ]
     => eapply plus2_star2 in H;
@@ -416,9 +346,9 @@ Ltac zsimpl_step :=
   | [ H : plus2 step ?σ1 nil ?σ2, H' : star2 step ?σ2 nil ?σ3
       |- sim_gen _ _ ?σ1 _ ]
     => pose proof (star2_trans (plus2_star2 H) H')
-  | [ SIM : sim' ?t ?σ1 ?σ2,
+  | [ SIM : sim bot3 ?t ?σ1 ?σ2,
             ACT : normal2 step ?σ2', STAR: star2 step ?σ2 nil ?σ2' |- _ ] =>
-    eapply sim'_reduction_closed_2 in SIM; [| eapply STAR]
+    eapply sim_reduction_closed_2 in SIM; [| eapply STAR]
   end.
 
 Ltac zzsimpl :=
@@ -428,29 +358,29 @@ Ltac zzcases :=
   match goal with
     [ H : plus2 (@step ?S ?ST) ?σ1 nil ?σ2a, H' : plus2 (@step ?S ?ST) ?σ1 nil ?σ2b |- _ ]
     => edestruct (plus2_reach H H' (@step_internally_deterministic _ ST))
-  | [ H: sim' _ ?σ1 ?σ2, H' : activated ?σ2 |- _ ] =>
+  | [ H: sim bot3 _ ?σ1 ?σ2, H' : activated ?σ2 |- _ ] =>
     match goal with
     | [ H : activated σ1 |- _ ] => fail 1
-    | _ => destruct (sim'_activated_2 H' H) as [? [? [[? [? ?]]| [? ?]]]]
+    | _ => destruct (sim_activated_2 H' H) as [? [? [[? [? ?]]| [? ?]]]]
     end
-  | [ H: sim' _ ?σ1 ?σ2, H' : activated ?σ1 |- _ ] =>
+  | [ H: sim bot3 _ ?σ1 ?σ2, H' : activated ?σ1 |- _ ] =>
     match goal with
     | [ H : activated σ2 |- _ ] => fail 1
-    | _ => destruct (sim'_activated H' H) as [? [? [? [? ?]]]]
+    | _ => destruct (sim_activated H' H) as [? [? [? [? ?]]]]
     end
   | [ STAR : star2 step ?σ2 nil ?σ2', NORM: normal2 step ?σ2',
                                             SIM : paco3 (@sim_gen _ _ _ _) bot3 _ ?σ1 ?σ2 |- _ ]
-    => edestruct (sim'_terminate_2 STAR NORM SIM) as [? [? [? [|]]]]
+    => edestruct (sim_terminate_2 STAR NORM SIM) as [? [? [? [|]]]]
   | [ STAR : star2 step ?σ1 nil ?σ1', NORM: normal2 step ?σ1',
                                             SIM : paco3 (@sim_gen _ _ _ _) bot3 _ ?σ1 ?σ2 |- _ ]
     => let H := fresh "H" in
       assert (result σ1' <> None) by congruence;
-      destruct (sim'_terminate STAR NORM H SIM) as [? [? [? ?]]];
+      destruct (sim_terminate STAR NORM H SIM) as [? [? [? ?]]];
       clear H
-  | [ NORM: normal2 step ?σ1, SIM : sim' _ ?σ1 ?σ2 |- _ ]
+  | [ NORM: normal2 step ?σ1, SIM : sim bot3 _ ?σ1 ?σ2 |- _ ]
     => let H := fresh "H" in
       assert (result σ1 <> None) by congruence;
-      destruct (sim'_terminate (@star2_refl _ _ σ1) NORM H SIM) as [? [? [? ?]]];
+      destruct (sim_terminate (@star2_refl _ _ σ1) NORM H SIM) as [? [? [? ?]]];
       clear H
   end.
 
@@ -464,24 +394,24 @@ Proof.
   eexists; eauto.
 Qed.
 
-Lemma sim'_t_Sim_activated t S1 `{StateType S1}
+Lemma sim_t_Sim_activated t S1 `{StateType S1}
       (σ1:S1)
   : result σ1 = ⎣⎦
     -> normal2 step σ1
     -> forall S2 `{StateType S2} (σ2:S2),
-        sim' t σ1 σ2
+        sim bot3 t σ1 σ2
         -> activated σ2
         -> t = Sim.
 Proof.
   intros. pinversion H3; subst; eauto; exfalso; relsimpl; eauto using plus_not_normal.
 Qed.
 
-Lemma sim'_t_Sim_normal t S1 `{StateType S1}
+Lemma sim_t_Sim_normal t S1 `{StateType S1}
       (σ1:S1) S2 `{StateType S2} (σ2:S2)
   : result σ1 = ⎣⎦
     -> normal2 step σ1
     -> normal2 step σ2
-    -> sim' t σ1 σ2
+    -> sim bot3 t σ1 σ2
     -> t = Sim \/ result σ2 = None.
 Proof.
   intros. pinversion H4; subst; eauto; relsimpl.
@@ -489,11 +419,11 @@ Proof.
   - right. congruence.
 Qed.
 
-Lemma sim'_t_Sim_normal_step t S1 `{StateType S1}
+Lemma sim_t_Sim_normal_step t S1 `{StateType S1}
       (σ1:S1) S2 `{StateType S2} (σ2:S2)
   : result σ1 = ⎣⎦
     -> normal2 step σ1
-    -> sim' t σ1 σ2
+    -> sim bot3 t σ1 σ2
     -> t = Sim \/ exists σ2', star2 step σ2 nil σ2' /\ normal2 step σ2' /\ result σ2' = None.
 Proof.
   intros. pinversion H3; subst; eauto; relsimpl.
@@ -514,12 +444,12 @@ end.
 Local Hint Resolve plus2_star2.
 
 
-Lemma sim'_zigzag t {S1} `{StateType S1}
+Lemma sim_zigzag t {S1} `{StateType S1}
       (σ1:S1) {S2} `{StateType S2} (σ2a σ2b:S2) {S3} `{StateType S3} (σ3:S3)
-  : sim' t σ1 σ2a
+  : sim bot3 t σ1 σ2a
     -> (star2 step σ2a nil σ2b \/ star2 step σ2b nil σ2a)
-    -> sim' t σ2b σ3
-    -> sim' t σ1 σ3.
+    -> sim bot3 t σ2b σ3
+    -> sim bot3 t σ1 σ3.
 Proof.
   revert σ1 σ2a σ2b σ3. pcofix CIH; intros.
   destruct H4.
@@ -534,7 +464,7 @@ Proof.
           * intros. zzsimpl; eauto 30 using star2_refl.
           * intros. zzsimpl; eauto 30 using star2_refl.
         + zzsimpl. assert (t = Sim).
-          eapply (@sim'_t_Sim_activated t _ _ _ H10 H9 _ _ _ H7); eauto.
+          eapply (@sim_t_Sim_activated t _ _ _ H10 H9 _ _ _ H7); eauto.
           subst.
           econstructor 3; eauto using plus2_star2, star2_trans.
       - (* plus step <-> err *)
@@ -548,7 +478,7 @@ Proof.
         + pfold. zzsimpl.
           econstructor 4; eauto; eauto.
         + zzsimpl.
-          destruct (@sim'_t_Sim_normal t _ _ _ _ _ _ H9 H8 H14 H7); eauto.
+          destruct (@sim_t_Sim_normal t _ _ _ _ _ _ H9 H8 H14 H7); eauto.
           * subst.
             pfold. econstructor 3; eauto using plus2_star2, star2_trans.
           * pfold. econstructor 4; eauto using plus2_star2, star2_trans.
@@ -575,7 +505,7 @@ Proof.
           econstructor 4; eauto. eauto.
         + zzsimpl.
           rewrite H4 in H10.
-          destruct (@sim'_t_Sim_normal_step _ _ _ _ _ _ _ H10 H9 H15); eauto.
+          destruct (@sim_t_Sim_normal_step _ _ _ _ _ _ _ H10 H9 H15); eauto.
           * subst.
             pfold. econstructor 3; eauto. congruence.
           * destruct H2; dcr.
@@ -600,7 +530,7 @@ Proof.
           * intros. zzsimpl; eauto 30 using star2_refl.
           * intros. zzsimpl; eauto 30 using star2_refl.
         + zzsimpl. assert (t = Sim).
-          eapply (@sim'_t_Sim_activated t _ _ _ H10 H9 _ _ _ H7); eauto.
+          eapply (@sim_t_Sim_activated t _ _ _ H10 H9 _ _ _ H7); eauto.
           subst.
           econstructor 3; eauto using plus2_star2, star2_trans.
       - (* plus step <-> err *)
@@ -614,7 +544,7 @@ Proof.
         + pfold. zzsimpl.
           econstructor 4; eauto; eauto.
         + zzsimpl.
-          destruct (@sim'_t_Sim_normal t _ _ _ _ _ _ H9 H8 H14 H7); eauto.
+          destruct (@sim_t_Sim_normal t _ _ _ _ _ _ H9 H8 H14 H7); eauto.
           * subst.
             pfold. econstructor 3; eauto using plus2_star2, star2_trans.
           * pfold. econstructor 4; eauto using plus2_star2, star2_trans.
@@ -641,7 +571,7 @@ Proof.
           econstructor 4; eauto; eauto.
         + zzsimpl.
           rewrite H4 in H10.
-          destruct (@sim'_t_Sim_normal_step _ _ _ _ _ _ _ H10 H9 H15); eauto.
+          destruct (@sim_t_Sim_normal_step _ _ _ _ _ _ _ H10 H9 H15); eauto.
           * subst.
             pfold. econstructor 3; eauto. congruence.
           * destruct H2; dcr.
@@ -658,23 +588,9 @@ Proof.
 Qed.
 
 
-Lemma sim'_trans t {S1} `{StateType S1}
-      (σ1:S1) {S2} `{StateType S2} (σ2:S2) {S3} `{StateType S3} (σ3:S3)
-  : sim' t σ1 σ2 -> sim' t σ2 σ3 -> sim' t σ1 σ3.
-Proof.
-  intros. eauto using (sim'_zigzag (S1:=S1) (S2:=S2) (S3:=S3)), star2_refl.
-Qed.
-
 Lemma sim_trans t {S1} `{StateType S1}
       (σ1:S1) {S2} `{StateType S2} (σ2:S2) {S3} `{StateType S3} (σ3:S3)
-  : sim t σ1 σ2
-    -> sim t σ2 σ3
-    -> sim t σ1 σ3.
+  : sim bot3 t σ1 σ2 -> sim bot3 t σ2 σ3 -> sim bot3 t σ1 σ3.
 Proof.
-  intros. eapply sim'_sim.
-  eapply sim_sim' in H2.
-  eapply sim_sim' in H3.
-  eapply (sim'_trans H2 H3).
+  intros. eauto using (sim_zigzag (S1:=S1) (S2:=S2) (S3:=S3)), star2_refl.
 Qed.
-
-Arguments sim_trans t [S1] {H} σ1 [S2] {H0} σ2 [S3] {H1} σ3 _ _.
