theories/Equiv/NonParametricBiSim.v
@@ -1,0 +1,214 @@
+Require Import List paco2.
+Require Import Util IL AllInRel Sawtooth.
+Require Export SmallStepRelations StateType Sim.
+
+Set Implicit Arguments.
+Unset Printing Records.
+
+(** * Non-parametric Definitions of Simulation and Bisimulation *)
+(** * Bisimulation *)
+(** A characterization of bisimulation equivalence on states;
+    works only for internally deterministic semantics. *)
+
+CoInductive bisim {S} `{StateType S} {S'} `{StateType S'}  : S -> S' -> Prop :=
+  | BisimSilent (σ1 σ1':S) (σ2 σ2':S') :
+      plus2 step σ1 nil σ1'
+      -> plus2 step σ2 nil σ2'
+      -> bisim σ1' σ2'
+      -> bisim σ1 σ2
+  | BisimExtern (pσ1 σ1:S) (pσ2 σ2:S') :
+      star2 step pσ1 nil σ1
+      -> star2 step pσ2 nil σ2
+      -> activated σ1
+      -> activated σ2
+      -> (forall evt σ1', step σ1 evt σ1' -> exists σ2', step σ2 evt σ2' /\ bisim σ1' σ2')
+      -> (forall evt σ2', step σ2 evt σ2' -> exists σ1', step σ1 evt σ1' /\ bisim σ1' σ2')
+      -> bisim pσ1 pσ2
+  | BisimTerm (σ1 σ1':S) (σ2 σ2':S')
+    : result σ1' = result σ2'
+      -> star2 step σ1 nil σ1'
+      -> star2 step σ2 nil σ2'
+      -> normal2 step σ1'
+      -> normal2 step σ2'
+      -> bisim σ1 σ2.
+
+Arguments bisim [S] {H} [S'] {H0} _ _.
+
+(** ** Bisimulation is an reflexive and symmetric *)
+Lemma bisim_refl {S} `{StateType S} (σ:S)
+      : bisim σ σ.
+Proof.
+  revert σ. cofix.
+  intros. destruct (step_dec σ) as [[[] []]|].
+  - eapply BisimExtern; intros; eauto using star2_refl; eexists; eauto.
+  - eapply BisimSilent; eauto using plus2O.
+  - eapply BisimTerm; eauto using star2_refl.
+Qed.
+
+Lemma bisim_sym {S} `{StateType S} {S'} `{StateType S'} (σ:S) (σ':S')
+      : bisim σ σ' -> bisim σ' σ.
+Proof.
+  revert σ σ'. cofix; intros.
+  inv H1.
+  - eapply BisimSilent; eauto.
+  - eapply BisimExtern; eauto; intros.
+    edestruct H7; eauto; dcr. eexists; eauto.
+    edestruct H6; eauto; dcr. eexists; eauto.
+  - eapply BisimTerm; eauto using star2_refl.
+Qed.
+
+Lemma bisim_simp t {S} `{StateType S} {S'} `{StateType S'}
+  : forall (σ:S) (σ':S'), bisim σ σ' -> sim bot3 t σ σ'.
+Proof.
+  pcofix CIH; intros. invt bisim; pfold; eauto using sim_gen.
+  - econstructor 2; eauto.
+    + intros. edestruct H6; eauto; dcr; eauto.
+    + intros. edestruct H7; eauto; dcr; eauto.
+Qed.
+
+Lemma simp_bisim {S} `{StateType S} {S'} `{StateType S'}
+  : forall (σ:S) (σ':S'), sim bot3 Bisim σ σ' -> bisim σ σ'.
+Proof.
+  cofix CIH; intros.
+  assert (sim_gen (paco3 (sim_gen (S:=S) (S':=S')) bot3 \3/ bot3) Bisim σ σ').
+  punfold H1.
+  inv H2; pclearbot.
+  - econstructor 1; eauto.
+  - econstructor 2; eauto.
+    + intros. edestruct H7; eauto; dcr; pclearbot; eauto.
+    + intros. edestruct H8; eauto; dcr; pclearbot; eauto.
+  - econstructor 3; eauto.
+Qed.
+
+Lemma bisim_trans {S1} `{StateType S1}
+      (σ1:S1) {S2} `{StateType S2} (σ2:S2) {S3} `{StateType S3} (σ3:S3)
+  : bisim σ1 σ2
+    -> bisim σ2 σ3
+    -> bisim σ1 σ3.
+Proof.
+  intros. eapply simp_bisim.
+  eapply bisim_simp in H2.
+  eapply bisim_simp in H3.
+  eapply (Sim.sim_trans H2 H3).
+Qed.
+
+(** ** Simulation *)
+
+CoInductive sim {S} `{StateType S} {S'} `{StateType S'}  : S -> S' -> Prop :=
+  | SimSilent (σ1 σ1':S) (σ2 σ2':S') :
+      plus2 step σ1 nil σ1'
+      -> plus2 step σ2 nil σ2'
+      -> sim σ1' σ2'
+      -> sim σ1 σ2
+  | SimExtern (pσ1 σ1:S) (pσ2 σ2:S') :
+      star2 step pσ1 nil σ1
+      -> star2 step pσ2 nil σ2
+      -> activated σ1
+      -> activated σ2
+      -> (forall evt σ1', step σ1 evt σ1' -> exists σ2', step σ2 evt σ2' /\ sim σ1' σ2')
+      -> (forall evt σ2', step σ2 evt σ2' -> exists σ1', step σ1 evt σ1' /\ sim σ1' σ2')
+      -> sim pσ1 pσ2
+  | SimTerm (σ1 σ1':S) (σ2 σ2':S')
+    : result σ1' = result σ2'
+      -> star2 step σ1 nil σ1'
+      -> star2 step σ2 nil σ2'
+      -> normal2 step σ1'
+      -> normal2 step σ2'
+      -> sim σ1 σ2
+  | SimErr (σ1 σ1':S) (σ2:S')
+    : result σ1' = None
+      -> star2 step σ1 nil σ1'
+      -> normal2 step σ1'
+      -> sim σ1 σ2.
+
+Arguments bisim [S] {H} [S'] {H0} _ _.
+
+(** ** Bisimulation is an reflexive and symmetric *)
+
+Lemma sim_refl {S} `{StateType S} (σ:S)
+      : sim σ σ.
+Proof.
+  revert σ. cofix.
+  intros. destruct (step_dec σ) as [[[] []]|].
+  - eapply SimExtern; intros; eauto using star2_refl; eexists; eauto.
+  - eapply SimSilent; eauto using plus2O.
+  - eapply SimTerm; eauto using star2_refl.
+Qed.
+
+Lemma sim_simp {S} `{StateType S} {S'} `{StateType S'}
+  : forall (σ:S) (σ':S'), sim σ σ' -> Sim.sim bot3 Sim σ σ'.
+Proof.
+  pcofix CIH; intros. inv H2; pfold; eauto using sim_gen.
+  - econstructor 2; eauto.
+    + intros. edestruct H6; eauto; dcr; eauto.
+    + intros. edestruct H7; eauto; dcr; eauto.
+Qed.
+
+Lemma simp_sim t {S} `{StateType S} {S'} `{StateType S'}
+  : forall (σ:S) (σ':S'), Sim.sim bot3 t σ σ' -> sim σ σ'.
+Proof.
+  cofix CIH; intros.
+  assert (sim_gen (paco3 (sim_gen (S:=S) (S':=S')) bot3 \3/ bot3) t σ σ').
+  punfold H1.
+  inversion H2; pclearbot.
+  - econstructor 1; eauto.
+  - econstructor 2; eauto.
+    + intros. edestruct H7; eauto; dcr; pclearbot; eauto.
+    + intros. edestruct H8; eauto; dcr; pclearbot; eauto.
+  - econstructor 4; eauto.
+  - econstructor 3; eauto.
+Qed.
+
+Lemma sim_trans {S1} `{StateType S1}
+      (σ1:S1) {S2} `{StateType S2} (σ2:S2) {S3} `{StateType S3} (σ3:S3)
+  : sim σ1 σ2
+    -> sim σ2 σ3
+    -> sim σ1 σ3.
+Proof.
+  intros. eapply simp_sim.
+  eapply sim_simp in H2.
+  eapply sim_simp in H3.
+  eapply (Sim.sim_trans H2 H3).
+Qed.
+
+Arguments sim_trans [S1] {H} σ1 [S2] {H0} σ2 [S3] {H1} σ3 _ _.
+
+
+(** Receptive and determinate according to CompCertTSO (Sevcík 2013)  *)
+
+Definition same_call (e e':extern) := extern_fnc e = extern_fnc e' /\ extern_args e = extern_args e'.
+
+Definition receptive S `{StateType S} :=
+  forall σ σ' ext, step σ (EvtExtern ext) σ'
+              -> forall ext', same_call ext ext' -> exists σ'', step σ (EvtExtern ext') σ''.
+
+Arguments receptive S [H].
+
+Definition determinate S `{StateType S} :=
+  forall σ σ' σ'' ext ext', step σ (EvtExtern ext) σ'
+              -> step σ (EvtExtern ext') σ'' -> same_call ext ext'.
+
+Arguments determinate S [H].
+
+Lemma bisimExternDet {S} `{StateType S} {S'} `{StateType S'} (pσ1:S) (pσ2:S') (σ1:S) (σ2:S')
+      (RCPT:receptive S) (DET:determinate S')
+: star2 step pσ1 nil σ1
+  -> star2 step pσ2 nil σ2
+  -> activated σ1
+  -> (forall evt σ1', step σ1 evt σ1' -> exists σ2', step σ2 evt σ2' /\ bisim σ1' σ2')
+  -> bisim pσ1 pσ2.
+Proof.
+  intros.
+  econstructor 2; eauto.
+  - inv H3. dcr. edestruct H4; eauto. firstorder.
+  - intros. inv H3. dcr. exploit H4; eauto; dcr.
+    destruct evt.
+    + exploit DET. eauto. eapply H5.
+      exploit RCPT; eauto. dcr.
+      exploit H4. eapply H11. dcr.
+      eexists; split. eapply H11.
+      exploit step_externally_determined. Focus 3.
+      instantiate (2:=σ2') in H8. rewrite H8. eapply H14.
+      eauto. eauto.
+    + exfalso. exploit step_internally_deterministic; eauto; dcr. congruence.
+Qed.
